src/Std/Tactic/BVDecide/Reflect.lean
@@ -126,8 +126,8 @@ theorem clz_congr (w : Nat) (x x' : BitVec w) (h : x = x') :
     BitVec.clz x' = BitVec.clz x := by
   simp [*]
 
-theorem popCount_congr (w : Nat) (x x' : BitVec w) (h : x = x') :
-    BitVec.popCount x' = BitVec.popCount x := by
+theorem cpop_congr (w : Nat) (x x' : BitVec w) (h : x = x') :
+    BitVec.cpop x' = BitVec.cpop x := by
   simp [*]
 
 end BitVec
